update the addtions to be closer to the values in the accumulator

dfy_model/MultiplyExpr256.dfy
@@ -29,11 +29,10 @@ module MultiplyExpr256 {
  	 	ensures flh(x) * B2 + flh(x) == x;
  	 	ensures flh(x) == x % B2;
 
-    method mul_limb(a: uint64, b: uint64)
-        returns (c: uint128)
-        ensures c as int == a as int * b as int;
+    function method mul_limb(a: uint64, b: uint64) : uint128
+        ensures mul_limb(a, b) == a as int * b as int;
     {
-        c := a as uint128 * b as uint128;
+        a as uint128 * b as uint128
     }
 
     function interp_wide(wr: wide_register) : int
@@ -46,24 +45,20 @@ module MultiplyExpr256 {
         ensures c_01 + c_23 * B2 + d_01 * B4 + d_23 * B6 ==
             interp_wide(a) * interp_wide(b);
     {
-        var p0 :uint128 := mul_limb(a[0], b[0]);
-        var p1 :uint128 := mul_limb(a[1], b[0]);
-        var p2 :uint128 := mul_limb(a[0], b[1]);
+        var a0 :uint256 := mul_limb(a[0], b[0]);
+        var a1 :uint256 := a0 + mul_limb(a[1], b[0]) * B;
+        var a2 :uint256 := a1 + mul_limb(a[0], b[1]) * B;
+        c_01 := lh(a2);
 
-        var t0 :uint256 := p0 + p1 * B + p2 * B;
-        c_01 := lh(t0);
+        var a3 :uint256 := uh(a2) + mul_limb(a[2], b[0]);
+        var a4 :uint256 := a3 + mul_limb(a[1], b[1]);
+        var a5 :uint256 := a4 + mul_limb(a[0], b[2]);
 
-        var p3 :uint128 := mul_limb(a[2], b[0]);
-        var p4 :uint128 := mul_limb(a[1], b[1]);
-        var p5 :uint128 := mul_limb(a[0], b[2]);
-
-        var p6 :uint128 := mul_limb(a[3], b[0]);
-        var p7 :uint128 := mul_limb(a[2], b[1]);
-        var p8 :uint128 := mul_limb(a[1], b[2]);
-        var p9 :uint128 := mul_limb(a[0], b[3]);
-
-        var t1 :uint256 := p3 + p4 + p5 + p6 * B + p7 * B + p8 * B + p9 * B + uh(t0);
-        c_23 := lh(t1);
+        var a6 :uint256 := a5 + mul_limb(a[3], b[0]) * B;
+        var a7 :uint256 := a6 + mul_limb(a[2], b[1]) * B;
+        var a8 :uint256 := a7 + mul_limb(a[1], b[2]) * B;
+        var a9 :uint256 := a8 + mul_limb(a[0], b[3]) * B;
+        c_23 := lh(a9);
 
         var p10 :uint128 := mul_limb(a[3], b[1]);
         var p11 :uint128 := mul_limb(a[2], b[2]);
@@ -72,7 +67,7 @@ module MultiplyExpr256 {
         var p13 :uint128 := mul_limb(a[3], b[2]);
         var p14 :uint128 := mul_limb(a[2], b[3]);
 
-        var t2 :uint256 := p10 + p11 + p12 + p13 * B + p14 * B + uh(t1);
+        var t2 :uint256 := p10 + p11 + p12 + p13 * B + p14 * B + uh(a9);
         d_01 := lh(t2);
 
         var p15 :uint128 := mul_limb(a[3], b[3]);
@@ -80,24 +75,24 @@ module MultiplyExpr256 {
 
         d_23 := lh(t3);
         assume d_23 == t3;
-        test_full_mul_lemma(a, b, t0, t1, t2, t3, c_01, c_23, d_01, d_23);
+        test_full_mul_lemma(a, b, a2, a9, t2, t3, c_01, c_23, d_01, d_23);
     }
 
     lemma test_full_mul_lemma(
         a : wide_register, b : wide_register,
-        t0 : uint256, t1 : uint256, t2 : uint256, t3 : uint256,
+        a2 : uint256, a9: uint256, t2 : uint256, t3 : uint256,
         c_01: uint128, c_23: uint128, d_01: uint128, d_23: uint128)
         
-        requires t0 == a[0] * b[0] + 
+        requires a2 == a[0] * b[0] + 
             a[1] * b[0] * B + a[0] * b[1] * B;
-        requires t1 == a[2] * b[0] + a[1] * b[1] + a[0] * b[2] +
-            a[3] * b[0] * B + a[2] * b[1] * B + a[1] * b[2] * B + a[0] * b[3] * B + uh(t0);
+        requires a9== a[2] * b[0] + a[1] * b[1] + a[0] * b[2] +
+            a[3] * b[0] * B + a[2] * b[1] * B + a[1] * b[2] * B + a[0] * b[3] * B + uh(a2);
         requires t2 == a[3] * b[1] + a[2] * b[2] + a[1] * b[3] + 
-            a[3] * b[2] * B + a[2] * b[3] * B + uh(t1);
+            a[3] * b[2] * B + a[2] * b[3] * B + uh(a9);
         requires t3 == a[3] * b[3] + uh(t2);
 
-        requires c_01 == lh(t0);
-        requires c_23 == lh(t1);
+        requires c_01 == lh(a2);
+        requires c_23 == lh(a9);
         requires d_01 == lh(t2);
         requires d_23 == t3;
 
@@ -112,8 +107,8 @@ module MultiplyExpr256 {
 
         var g2 :int := a[3] as int * b[3];
 
-        assert t1 == g0 + uh(t0);
-        assert t2 == g1 + uh(t1);
+        assert a9== g0 + uh(a2);
+        assert t2 == g1 + uh(a9);
         assert t3 == g2 + uh(t2);
 
         calc == {
@@ -125,31 +120,31 @@ module MultiplyExpr256 {
                 assume lh(t2) * B4 + uh(t2) * B6 == t2 * B4;
             }
             c_01 + c_23 * B2 + t2 * B4 + g2 * B6;
-            c_01 + lh(t1) * B2 + t2 * B4 + g2 * B6;
-            c_01 + lh(t1) * B2 + (g1 + uh(t1)) * B4 + g2 * B6;
-            c_01 + lh(t1) * B2 + g1 * B4 + uh(t1) * B4 + g2 * B6;
+            c_01 + lh(a9) * B2 + t2 * B4 + g2 * B6;
+            c_01 + lh(a9) * B2 + (g1 + uh(a9)) * B4 + g2 * B6;
+            c_01 + lh(a9) * B2 + g1 * B4 + uh(a9) * B4 + g2 * B6;
             {
-                assume lh(t1) * B2 + uh(t1) * B4 == t1 * B2;
+                assume lh(a9) * B2 + uh(a9) * B4 == a9* B2;
             }
-            c_01 + t1 * B2 + g1 * B4 + g2 * B6;
-            lh(t0) + t1 * B2 + g1 * B4 + g2 * B6;
-            lh(t0) + (g0 + uh(t0)) * B2 + g1 * B4 + g2 * B6;
-            lh(t0) + g0 * B2 + uh(t0) * B2 + g1 * B4 + g2 * B6;
+            c_01 + a9* B2 + g1 * B4 + g2 * B6;
+            lh(a2) + a9* B2 + g1 * B4 + g2 * B6;
+            lh(a2) + (g0 + uh(a2)) * B2 + g1 * B4 + g2 * B6;
+            lh(a2) + g0 * B2 + uh(a2) * B2 + g1 * B4 + g2 * B6;
             {
-                assume lh(t0) + uh(t0) * B2 == t0;
+                assume lh(a2) + uh(a2) * B2 == a2;
             }
-            t0 + g0 * B2 + g1 * B4 + g2 * B6;
+            a2 + g0 * B2 + g1 * B4 + g2 * B6;
             {
-                test_full_mul_aux_lemma(a, b, t0, g0, g1, g2);
+                test_full_mul_aux_lemma(a, b, a2, g0, g1, g2);
             }
             interp_wide(a) * interp_wide(b);
         }
     }
 
     lemma test_full_mul_aux_lemma(a: wide_register, b: wide_register,
-        t0: int, g0: int, g1: int, g2: int)
+        a2: int, g0: int, g1: int, g2: int)
 
-        requires t0 == a[0] * b[0] + 
+        requires a2 == a[0] * b[0] + 
             a[1] * b[0] * B + a[0] * b[1] * B;
         requires g0 == a[2] * b[0] + a[1] * b[1] + a[0] * b[2] +
             a[3] * b[0] * B + a[2] * b[1] * B + a[1] * b[2] * B + a[0] * b[3] * B;
@@ -157,7 +152,7 @@ module MultiplyExpr256 {
             a[3] * b[2] * B + a[2] * b[3] * B;
         requires g2 == a[3] as int * b[3];
 
-        ensures interp_wide(a) * interp_wide(b) == t0 + g0 * B2 + g1 * B4 + g2 * B6;
+        ensures interp_wide(a) * interp_wide(b) == a2 + g0 * B2 + g1 * B4 + g2 * B6;
     {
         assert true;
     }
